dsn/Lang/Dynamic/Confluent.lean
@@ -1,6 +1,6 @@
 import Lang.Basic
-import Lang.Dynamic.Transition
 import Lang.Dynamic.EvalCon
+import Lang.Dynamic.Transition
 import Lang.Dynamic.TransitionStar
 import Lang.Dynamic.Convergent
 import Lang.Dynamic.Divergent
