dsn/Lang/Dynamic/Safe.lean
@@ -1,0 +1,89 @@
+import Lang.Basic
+import Lang.Dynamic.EvalCon
+import Lang.Dynamic.Transition
+import Lang.Dynamic.TransitionStar
+import Lang.Dynamic.Convergent
+import Lang.Dynamic.Divergent
+
+set_option pp.fieldNotation false
+
+
+namespace Lang.Dynamic
+
+
+mutual
+  inductive RecSafe : List (String × Expr) → Prop
+  | nil : RecSafe []
+  | cons l e r :
+    List.is_fresh_key l r → Safe e →
+    RecSafe r → RecSafe ((l,e)::r)
+
+  inductive Safe : Expr → Prop
+  | convergent e : Convergent e → Safe e
+  | iso l body : Safe body → Safe (.iso l body)
+  | record r : RecSafe r → Safe (.record r)
+  | function f : Safe (.function f)
+  | app e e' : Safe e → Safe e' → Safe (.app e e')
+  | loop e : Divergent (.loop e) → Safe (.loop e)
+end
+
+
+theorem Safe.subject_reduction :
+  Transition e e' →
+  Safe e →
+  Safe e'
+:= by sorry
+
+theorem Safe.subject_expansion :
+  Transition e e' →
+  Safe e' →
+  Safe e
+:= by sorry
+
+mutual
+
+  theorem Safe.evalcon_preservation
+    (evalcon : EvalCon E)
+    (safe_evalcon : Safe (E e))
+  : Safe e' → Safe (E e')
+  := by cases evalcon with
+  | hole =>
+    intro h0
+    simp
+    exact h0
+  | iso l econ =>
+    intro h0
+    simp
+    simp at safe_evalcon
+    have econ' := EvalCon.iso l econ
+    apply Safe.evalcon_preservation econ' safe_evalcon h0
+  -- | record : RecordCon R → EvalCon (fun e => .record (R e))
+  -- | applicator e' : EvalCon E → EvalCon (fun e => .app (E e) e')
+  -- | applicand f : EvalCon E → EvalCon (fun e => .app (.function f) (E e))
+  -- | loopy : EvalCon E → EvalCon (fun e => Expr.loop (E e))
+  | _ => sorry
+  termination_by sizeOf evalcon
+  decreasing_by sorry
+
+  -- inductive RecordCon : (Expr → List (String × Expr)) → Prop
+  -- | head l r :  EvalCon E → RecordCon (fun e => (l, E e) :: r)
+  -- | tail l :
+  --     RecordCon R →
+  --     Expr.is_value ev →
+  --     RecordCon (fun e => (l,ev) :: (R e))
+
+theorem Safe.evalcon_reflection :
+  EvalCon E →
+  Safe (E e) →
+  Safe e
+:= by
+  sorry
+
+end
+
+
+
+
+
+
+end Lang.Dynamic
